generic/Zeta.GenericVerifier.fsti
@@ -14,7 +14,26 @@ val hoist_ghost (#a:Type) (#b:a -> Type) (f:(x:a -> GTot (b x)))
   : GTot (g:(x:a -> b x){forall x. f x == g x})
 
 val hoist_ghost2 (#a:Type) (#b:a -> Type) (#c:(x:a -> b x -> Type)) (f:(x:a -> y:b x -> GTot (c x y)))
-  : GTot (g:(x:a -> y:b x -> c x y){forall x y. f x y == g x y})
+  : GTot (x:a -> y:b x -> c x y)
+
+val hoist_ghost2_apply (#a:Type) (#b:a -> Type) (#c:(x:a -> b x -> Type)) (f:(x:a -> y:b x -> GTot (c x y)))
+  (x:a) (y:b x)
+  : Lemma ((hoist_ghost2 f) x y == f x y)
+          [SMTPat ((hoist_ghost2 f) x y)]
+
+// let hoist_ghost_preserves_pred (#a:Type) (#b:a -> Type)
+//   (f:(x:a -> GTot (b x)))
+//   (pred:(x:a -> b x) -> Type0)
+//   : Lemma
+//       (requires
+//         (
+//       (ensures pred g <==> pred (hoist_ghost f))
+//   = ()
+
+// let hoist_ghost2_preserves_pred (#a:Type) (#b:a -> Type) (#c:(x:a -> b x -> Type))
+//   (f:(x:a -> y:b -> GTot (c x y)))
+//   (g:(x:a -> y:b -> c x y))
+  
 
 
 (* identifier type for verifier threads *)
